

$$F_X(x) = \int_{-\infty}^x \frac{1}{[0,1]} dx = \begin{cases} 1 & \text{si } x > 0 \\ 0 & \text{si } x \leq 0 \end{cases}$$

$$\begin{aligned} F_Y &= \frac{3}{8} \int_0^1 (1+xy+y^2) \frac{1}{[-1,1]} dx \\ &= \frac{3}{8} \frac{1}{[-1,1]} \left[ x + \frac{x^2 y}{2} + x y^2 \right]_0^1 = \\ &= \frac{3}{8} \left( y^2 + \frac{1}{2} y + 1 \right) \frac{1}{[-1,1]} \end{aligned}$$

$$F_Y(y) = \int_{-\infty}^y \frac{3}{8} \left( y^2 + \frac{1}{2} y + 1 \right) \frac{1}{[-1,1]} dy$$

$$= \begin{cases} 1 & \text{si } y > 1 \\ \frac{3}{8} \left( \frac{y^3}{3} + \frac{1}{4} y^2 + y \right) & \text{si } -1 < y < 1 \\ 0 & \text{si } y < -1 \end{cases}$$

3.  $X$  est une variable aléatoire constante sur  $[0,1]$

$$E_X = \int_{\mathbb{R}} x \frac{1}{[0,1]} dx = \int_0^1 x dx = \left[ \frac{x^2}{2} \right]_0^1 = \frac{1}{2} \checkmark$$

$$\text{Var}(Y) = E(Y^2) - E(Y)^2$$

$$E(Y^2) \stackrel{\text{transf}}{=} \int_{\mathbb{R}} y^2 \frac{3}{8} \left( y^2 + \frac{1}{2} y + 1 \right) \frac{1}{[-1,1]} dy = \frac{3}{8} \int_{-1}^1 y^4 + \frac{1}{2} y^3 + y^2 dy$$

$$= \frac{3}{8} \left[ \frac{y^5}{5} + \frac{1}{8} y^4 + \frac{y^3}{3} \right]_{-1}^1 = \frac{3}{8} \left( \frac{1}{5} + \frac{1}{8} + \frac{1}{3} \right) - \left( \frac{-1}{5} + \frac{1}{8} - \frac{1}{3} \right) \\ = \frac{3}{8} \left( \frac{2}{5} + \frac{2}{3} \right) = \frac{3}{8} \times \frac{16}{15} = \frac{2}{5}$$

$$E(Y) = \int_{\mathbb{R}} y \frac{3}{8} \left( y^2 + \frac{1}{2} y + 1 \right) \frac{1}{[-1,1]} dy = \frac{3}{8} \int_{-1}^1 y^3 + \frac{1}{2} y^2 + y dy$$

$$= \frac{3}{8} \left[ \frac{y^4}{4} + \frac{1}{6} y^3 + \frac{y^2}{2} \right]_{-1}^1 = \frac{3}{8} \left( \frac{1}{4} + \frac{1}{6} + \frac{1}{2} \right) - \left( \frac{1}{4} - \frac{1}{6} + \frac{1}{2} \right) \\ = \frac{3}{8} \times \frac{2}{3} = \frac{1}{4} \checkmark, \text{Var}(Y) = \frac{2}{5} - \left( \frac{1}{4} \right)^2$$

